LeanCats/Basic.lean
@@ -1,0 +1,18 @@
+import LeanCats.Data
+import LeanCats.Relations
+
+open Data
+open CatRel
+
+/-- Each execution is abstracted to a candidate execution 〈evts , po, rf, co, IW, sr〉 providing
+This definination is different with the formal semantics, because the `co` is defined in [stdlib.cat](https://github.com/herd/herdtools7/blob/2a7599f8ecdbde0ed67925daf6534c1a0c26d535/herd-www/cat_includes/stdlib.cat) and
+by computation, so should declare it as the base relation. -/
+structure CandidateExecution
+  (evts : Events)
+  [IsStrictTotalOrder Event (preCo evts)]
+  where
+  (evts : Events)
+  (_po : Rel Event Event)
+  (_rf : Rel Event Event)
+  (_fr : Rel Event Event)
+  (_IW : Set Event)
