LeanCats/Data.lean
@@ -56,14 +56,4 @@ structure Events where
 instance : Membership Event Events where
   mem evts evt := evt ∈ evts.B ∪ evts.F ∪ evts.IW ∪ evts.R ∪ evts.RMW ∪ evts.W
 
-/-- Each execution is abstracted to a candidate execution 〈evts , po, rf, co, IW, sr〉 providing
-This definination is different with the formal semantics, because the `co` is defined in [stdlib.cat](https://github.com/herd/herdtools7/blob/2a7599f8ecdbde0ed67925daf6534c1a0c26d535/herd-www/cat_includes/stdlib.cat) and
-by computation, so should declare it as the base relation. -/
-structure CandidateExecution where
-  (evts : Events)
-  (po : Rel Event Event)
-  (rf : Rel Event Event)
-  (fr : Rel Event Event)
-  (IW : Set Event)
-
 end Data
