LeanCats/Syntax.lean
@@ -1,5 +1,3 @@
-namespace CatGrammar
-
 declare_syntax_cat dsl_term
 declare_syntax_cat expr
 declare_syntax_cat inst
@@ -16,94 +14,98 @@ declare_syntax_cat constraint
 declare_syntax_cat annotable_events
 declare_syntax_cat predefined_events
 declare_syntax_cat predefined_relations
+declare_syntax_cat cat_ident
 
-scoped syntax reserved : expr
-scoped syntax primitive : reserved
-scoped syntax keyword : reserved
-scoped syntax name : reserved
-scoped syntax predefined_events : reserved
-scoped syntax predefined_relations : reserved
+syntax reserved:41 : expr
+syntax primitive : reserved
+syntax keyword : reserved
+syntax name : reserved
+syntax predefined_events : reserved
+syntax predefined_relations : reserved
 
-scoped syntax "and" : keyword
-scoped syntax "as" : keyword
-scoped syntax "begin" : keyword
-scoped syntax "call" : keyword
-scoped syntax "do" : keyword
-scoped syntax "end" : keyword
-scoped syntax "enum" : keyword
-scoped syntax "flag" : keyword
-scoped syntax "forall" : keyword
-scoped syntax "from" : keyword
-scoped syntax "fun" : keyword
-scoped syntax "in" : keyword
-scoped syntax "instructions" : keyword
-scoped syntax "let" : keyword
-scoped syntax "match" : keyword
-scoped syntax "procedure" : keyword
-scoped syntax "rec" : keyword
-scoped syntax "scopes" : keyword
-scoped syntax "with" : keyword
+syntax "and" : keyword
+syntax "as" : keyword
+syntax "begin" : keyword
+syntax "call" : keyword
+syntax "do" : keyword
+syntax "end" : keyword
+syntax "enum" : keyword
+syntax "flag" : keyword
+syntax "forall" : keyword
+syntax "from" : keyword
+syntax "fun" : keyword
+syntax "in" : keyword
+syntax "instructions" : keyword
+syntax "let" : keyword
+syntax "match" : keyword
+syntax "procedure" : keyword
+syntax "rec" : keyword
+syntax "scopes" : keyword
+syntax "with" : keyword
 
-scoped syntax "classes" : primitive
-scoped syntax "linearizations" : primitive
-scoped syntax "tag2events" : primitive
-scoped syntax "tag2scopes" : primitive
+syntax "classes" : primitive
+syntax "linearizations" : primitive
+syntax "tag2events" : primitive
+syntax "tag2scopes" : primitive
 
-scoped syntax assertion : keyword
-scoped syntax "irreflexive" : assertion
-scoped syntax "empty" : assertion
-scoped syntax "acyclic" : assertion
+syntax assertion : keyword
+syntax "irreflexive" : assertion
+syntax "empty" : assertion
+syntax "acyclic" : assertion
 
-scoped syntax "_" : name
-scoped syntax "O" : name
-scoped syntax "ext" : name
-scoped syntax "FW" : name
-scoped syntax "id" : name
-scoped syntax "loc" : name
-scoped syntax "narrower" : name
-scoped syntax "wider" : name
+syntax "_" : name
+syntax "O" : name
+syntax "ext" : name
+syntax "FW" : name
+syntax "id" : name
+syntax "loc" : name
+syntax "narrower" : name
+syntax "wider" : name
 
--- annotable events.
-scoped syntax "W" : annotable_events -- write events
-scoped syntax "R" : annotable_events -- read events
-scoped syntax "B" : annotable_events -- branch events
-scoped syntax "F" : annotable_events -- fence events
+/- table events. -/
+syntax "W" : annotable_events -- write events
+syntax "R" : annotable_events -- read events
+syntax "B" : annotable_events -- branch events
+syntax "F" : annotable_events -- fence events
 
-scoped syntax "___" : predefined_events -- all events
-scoped syntax "IW" : predefined_events -- initial writes
-scoped syntax "M" : predefined_events -- memory events, M = W ∪ R
-scoped syntax annotable_events : predefined_events
+syntax "___" : predefined_events -- all events
+syntax "IW" : predefined_events -- initial writes
+syntax "M" : predefined_events -- memory events, M = W ∪ R
+syntax annotable_events : predefined_events
 
-/-- predefined_relations: -/
-scoped syntax "O" : predefined_relations -- empty relation
-scoped syntax "rf" : predefined_relations -- read from
-scoped syntax "fr" : predefined_relations -- from read
-scoped syntax "id" : predefined_relations -- identity
-scoped syntax "loc" : predefined_relations -- same location
-scoped syntax "ext" : predefined_relations -- external (different pids)
-scoped syntax "po" : predefined_relations -- program order
-scoped syntax "rmw" : predefined_relations -- read-modify-write
+/- defined_relations: -/
+syntax "O" : predefined_relations -- empty relation
+syntax "rf" : predefined_relations -- read from
+syntax "rfe" : predefined_relations -- read from external
+syntax "fr" : predefined_relations -- from read
+syntax "co" : predefined_relations -- from read
+syntax "id" : predefined_relations -- identity
+syntax "loc" : predefined_relations -- same location
+syntax "ext" : predefined_relations -- external (different pids)
+syntax "po" : predefined_relations -- program order
+syntax "rmw" : predefined_relations -- read-modify-write
 
-scoped syntax keyword : dsl_term
-scoped syntax num : dsl_term
-scoped syntax ident : dsl_term
-scoped syntax "(" expr ")" : dsl_term
+syntax keyword : dsl_term
+syntax num : dsl_term
+syntax "(" expr ")" : dsl_term
+syntax cat_ident : dsl_term
 
-scoped syntax dsl_term : expr
+syntax ident : cat_ident
+syntax ident"-"ident : cat_ident
 
-scoped syntax:50 expr:50 "|" expr:51 : expr
-scoped syntax expr "&" expr : expr
-scoped syntax expr ";" expr : expr
-scoped syntax:60 expr:60 "*" expr:61 : expr
-scoped syntax expr "^" expr : expr
-scoped syntax expr "+" expr : expr
-scoped syntax expr "-" expr : expr
-scoped syntax:71 expr "^-1" : expr
+syntax dsl_term:51 : expr
 
-scoped syntax assertion expr ("as" ident)? : inst
-scoped syntax "let" ident "=" expr : inst
+syntax:51 expr:51 "|" expr:50 : expr
+syntax expr "&" expr : expr
+syntax expr ";" expr : expr
+syntax:60 expr:60 "*" expr:61 : expr
+syntax expr "^" expr : expr
+syntax expr "+" expr : expr
+syntax expr "-" expr : expr
+syntax:71 expr "^-1" : expr
 
-scoped syntax "(*" ident* "*)" : inst
-scoped syntax "include" str : inst
+syntax assertion expr ("as" cat_ident)? : inst
+syntax "let" cat_ident "=" expr : inst
 
-end CatGrammar
+syntax "(*" ident* "*)" : inst
+syntax "include" str : inst
